code/src/internal/Gdt/eval.lean
@@ -48,14 +48,14 @@ end
 lemma Gdt.eval_rhs { rhs: Rhs } { env: Env }: (Gdt.rhs rhs).eval env = Result.value rhs :=
 by simp [Gdt.eval]
 
-lemma Gdt.eval_xgrd_of_some { xgrd: XGrd } { tr: Gdt } { env env': Env }
-    (h: xgrd_eval xgrd env = some env'):
-    (Gdt.grd (Grd.xgrd xgrd) tr).eval env = tr.eval env' :=
+lemma Gdt.eval_tgrd_of_some { tgrd: TGrd } { tr: Gdt } { env env': Env }
+    (h: tgrd_eval tgrd env = some env'):
+    (Gdt.grd (Grd.tgrd tgrd) tr).eval env = tr.eval env' :=
 by simp [Gdt.eval, Grd.eval, Result.bind, h]
 
-lemma Gdt.eval_xgrd_of_none { xgrd: XGrd } { tr: Gdt } { env: Env }
-    (h: xgrd_eval xgrd env = none):
-    (Gdt.grd (Grd.xgrd xgrd) tr).eval env = Result.no_match :=
+lemma Gdt.eval_tgrd_of_none { tgrd: TGrd } { tr: Gdt } { env: Env }
+    (h: tgrd_eval tgrd env = none):
+    (Gdt.grd (Grd.tgrd tgrd) tr).eval env = Result.no_match :=
 by simp [Gdt.eval, Grd.eval, Result.bind, h]
 
 lemma Gdt.eval_bang_of_bottom { var: Var } { tr: Gdt } { env: Env }
@@ -87,10 +87,10 @@ begin
     },
     case Gdt.grd {
         cases gdt_grd,
-        case Grd.xgrd {
-            cases c: xgrd_eval gdt_grd env,
-            { finish [Gdt.rhss, Gdt.eval_xgrd_of_none c, Gdt.eval, Grd.eval, Result.bind], },
-            { finish [Gdt.rhss, Gdt.eval_xgrd_of_some c, Gdt.eval, Grd.eval, Result.bind], },
+        case Grd.tgrd {
+            cases c: tgrd_eval gdt_grd env,
+            { finish [Gdt.rhss, Gdt.eval_tgrd_of_none c, Gdt.eval, Grd.eval, Result.bind], },
+            { finish [Gdt.rhss, Gdt.eval_tgrd_of_some c, Gdt.eval, Grd.eval, Result.bind], },
         },
         case Grd.bang {
             cases c: is_bottom gdt_grd env,
