code/src/internal/Gdt/mark_all_rhss_inactive.lean
@@ -47,12 +47,12 @@ lemma Gdt.mark_all_rhss_inactive_is_reduntant_set (gdt: Gdt) (rhss: finset Rhs):
 by simp [Ant.is_redundant_set, finset.inter_subset_right]
 
 
-lemma Gdt.mark_inactive_rhss_of_xgrd_some { xgrd: XGrd } { env env': Env } (h: xgrd_eval xgrd env = some env') (gdt: Gdt):
-    (Gdt.grd (Grd.xgrd xgrd) gdt).mark_inactive_rhss env = gdt.mark_inactive_rhss env' :=
+lemma Gdt.mark_inactive_rhss_of_tgrd_some { tgrd: TGrd } { env env': Env } (h: tgrd_eval tgrd env = some env') (gdt: Gdt):
+    (Gdt.grd (Grd.tgrd tgrd) gdt).mark_inactive_rhss env = gdt.mark_inactive_rhss env' :=
 by simp [Gdt.mark_inactive_rhss, h, Gdt.mark_inactive_rhss._match_1]
 
-lemma Gdt.mark_inactive_rhss_of_xgrd_none { xgrd: XGrd } { env: Env } (h: xgrd_eval xgrd env = none) (gdt: Gdt):
-    (Gdt.grd (Grd.xgrd xgrd) gdt).mark_inactive_rhss env = gdt.mark_all_rhss_inactive :=
+lemma Gdt.mark_inactive_rhss_of_tgrd_none { tgrd: TGrd } { env: Env } (h: tgrd_eval tgrd env = none) (gdt: Gdt):
+    (Gdt.grd (Grd.tgrd tgrd) gdt).mark_inactive_rhss env = gdt.mark_all_rhss_inactive :=
 by simp [Gdt.mark_inactive_rhss, h, Gdt.mark_inactive_rhss._match_1]
 
 lemma Gdt.mark_inactive_rhss_map_tt (gdt: Gdt) (env: Env):
@@ -61,7 +61,7 @@ begin
     induction gdt generalizing env;
     try { cases gdt_grd };
     try { cases c: (gdt_tr1.eval env).is_match };
-    try { cases c: (xgrd_eval gdt_grd env) };
+    try { cases c: (tgrd_eval gdt_grd env) };
     try { cases c: is_bottom gdt_grd env };
     simp [*, Gdt.rhss, Gdt.mark_inactive_rhss, Gdt.mark_all_rhss_inactive, Ant.map],
 end
@@ -73,7 +73,7 @@ begin
     induction gdt generalizing env;
     try { cases gdt_grd };
     try { cases c: (gdt_tr1.eval env).is_match };
-    try { cases c: (xgrd_eval gdt_grd env) };
+    try { cases c: (tgrd_eval gdt_grd env) };
     try { cases c: is_bottom gdt_grd env };
     simp [*, Gdt.rhss, Gdt.mark_inactive_rhss, Ant.critical_rhs_sets],
 end
@@ -94,11 +94,11 @@ begin
     },
     case Gdt.grd {
         cases gdt_grd with gdt_grd var,
-        case Grd.xgrd {
-            cases c: xgrd_eval gdt_grd env, {
+        case Grd.tgrd {
+            cases c: tgrd_eval gdt_grd env, {
                 simp [Gdt.mark_inactive_rhss, Gdt.mark_all_rhss_inactive, c],
             }, {
-                rw [Gdt.eval_xgrd_of_some c] at h,
+                rw [Gdt.eval_tgrd_of_some c] at h,
                 simp [Gdt.mark_inactive_rhss, Gdt.mark_all_rhss_inactive, c, gdt_ih h],
             },
         },
