code/src/internal/phi/eval.lean
@@ -20,20 +20,20 @@ begin
     simp [Φ.eval, c1, c2],
 end
 
-lemma Φ_eval_not_xgrd_some { gdt_grd: XGrd } { env env': Env } (h: xgrd_eval gdt_grd env = some env'):
-    (Φ.not_xgrd gdt_grd).eval env = ff :=
+lemma Φ_eval_not_tgrd_some { gdt_grd: TGrd } { env env': Env } (h: tgrd_eval gdt_grd env = some env'):
+    (Φ.not_tgrd gdt_grd).eval env = ff :=
 by simp [Φ.eval, h]
 
-lemma Φ_eval_not_xgrd_none { gdt_grd: XGrd } { env: Env } (h: xgrd_eval gdt_grd env = none):
-    (Φ.not_xgrd gdt_grd).eval env = tt :=
+lemma Φ_eval_not_tgrd_none { gdt_grd: TGrd } { env: Env } (h: tgrd_eval gdt_grd env = none):
+    (Φ.not_tgrd gdt_grd).eval env = tt :=
 by simp [Φ.eval, h]
 
-lemma Φ_eval_xgrd_some { gdt_grd: XGrd } { env env': Env } (h: xgrd_eval gdt_grd env = some env') (ty: Φ):
-    (Φ.xgrd_in gdt_grd ty).eval env = ty.eval env' :=
+lemma Φ_eval_tgrd_some { gdt_grd: TGrd } { env env': Env } (h: tgrd_eval gdt_grd env = some env') (ty: Φ):
+    (Φ.tgrd_in gdt_grd ty).eval env = ty.eval env' :=
 by simp [Φ.eval, h]
 
-lemma Φ_eval_xgrd_none { gdt_grd: XGrd } { env: Env } (h: xgrd_eval gdt_grd env = none) (ty: Φ):
-    (Φ.xgrd_in gdt_grd ty).eval env = ff :=
+lemma Φ_eval_tgrd_none { gdt_grd: TGrd } { env: Env } (h: tgrd_eval gdt_grd env = none) (ty: Φ):
+    (Φ.tgrd_in gdt_grd ty).eval env = ff :=
 by simp [Φ.eval, h]
 
 @[simp]
