code/src/internal/phi/utils.lean
@@ -18,7 +18,7 @@ lemma stable.id: stable id := by simp [stable]
 lemma stable.and_left { ty: Φ }: stable (λ ty', ty'.and ty) := by stable_macro
 lemma stable.and_right { ty: Φ }: stable ty.and := by stable_macro
 lemma stable.or_right { ty: Φ }: stable ty.or := by stable_macro
-lemma stable.xgrd_in (xgrd: XGrd): stable (Φ.xgrd_in xgrd) := by stable_macro
+lemma stable.tgrd_in (tgrd: TGrd): stable (Φ.tgrd_in tgrd) := by stable_macro
 
 lemma stable.app { f: Φ → Φ } (f_stable: stable f) { ty1 ty2: Φ } (h: ty1.eval = ty2.eval): (f ty1).eval = (f ty2).eval :=
 by finish [stable]
@@ -58,13 +58,13 @@ begin
     simp [*, Φ.eval],
 end
 
-lemma hom.xgrd_in (grd: XGrd): hom (Φ.xgrd_in grd) :=
+lemma hom.tgrd_in (grd: TGrd): hom (Φ.tgrd_in grd) :=
 begin
     rw hom,
     assume ty1 ty2,
     split;
     ext env;
-    cases c: xgrd_eval grd env;
+    cases c: tgrd_eval grd env;
     simp [*, Φ.eval],
 end
 
